proof/old_system/uni/def_ott.v
@@ -1417,6 +1417,8 @@ Inductive d_sub : denv -> typ -> typ -> Prop :=    (* defn d_sub *)
      d_sub Ψ A2 B2 ->
      d_sub Ψ (typ_arrow A1 A2) (typ_arrow B1 B2)
  | d_sub__all : forall (L:vars) (Ψ:denv) (A B:typ),
+      ( forall X , X \notin  L  -> d_sneq_stvar  ( X ~ dbind_tvar_empty  ++  Ψ )   ( open_typ_wrt_typ A (typ_var_f X) )  )  ->
+      ( forall X , X \notin  L  -> d_sneq_stvar  ( X ~ dbind_tvar_empty  ++  Ψ )   ( open_typ_wrt_typ B (typ_var_f X) )  )  ->
       ( forall X , X \notin  L  -> d_sub  ( X ~ dbind_stvar_empty  ++  Ψ )   ( open_typ_wrt_typ A (typ_var_f X) )   ( open_typ_wrt_typ B (typ_var_f X) )  )  ->
      d_sub Ψ (typ_all A) (typ_all B)
  | d_sub__alll : forall (L:vars) (Ψ:denv) (A B T:typ),
